\documentclass[a4paper]{article}

% --- DATA ---

\def\lecture{Operator Algebras}
\def\authors{Linus Mußmächer, Minona Schäfer}
\def\sheetNumber{04}
%\def\sumPoints{30} 

% --- PREAMBLE ---

\usepackage[english]{babel}	% language specific quotation marks etc.
\input{../../preambles/exercise_preamble.tex}

% --- DOCUMENT ---

\begin{document}

\makeexheader

\begin{center}
    \includegraphics*[width=0.4\textwidth]{pi.png}
\end{center}

\subsection{}

The first statement follows immediately from the fact that the canonical inclusion $\algebra{B} \hookrightarrow \algebra{A}$ is an injective $^*$-homomorphism, so it is isometric as proven in the lecture.

If now $\algebra{B}$ is a dense proper $^*$-subalgebra of $\algebra{A}$, assuming it could be turned into a $C^*$-algebra, the norm on that $C^*$-algebra would already have to be the norm on $\algebra{A}$.
But then the canonical inclusion is isometric and injective, so it has closed range and $\algebra{B} \subseteq \algebra{A}$ is closed and dense in $\algebra{A}$.
Now, however, we have $\algebra{B} = \algebra{A}$, a contradiction.

\subsection{}

As hinted, the disk algebra $\algebra{A}(\mathds{D})$ is such an algebra.
As we have $\overline{\overline{z}} = z$ for all $z \in \mathds{D}$, the identity map is self-adjoint, but because of $\frac{i}{2} \in \id(\mathds{D})$, $\id - \frac{i}{2} \cdot 1$ is not invertible.
Thus, $\frac{i}{2} \in \sigma(\id) \subsetneq \mathds{R}$.

Analogously, we can also consider the character $\phi: \algebra{A}(\mathds{D}) \to \mathds{C}: f \mapsto f\left(\frac{i}{2}\right)$.
Here, we have $\phi(\id^*) = \phi(\id) = \frac{i}{2} \neq - \frac{i}{2} = \overline{\phi(\id)}$.

\begin{enumerate}
    \item $\then$ (ii): Take $a \in \algebra{A}$ be any self-adjoint element and $(a)$ the $^*$-subalgebra generated by $a$ in $\algebra{A}$.
    Then $\Omega((a)) \subseteq \Omega(\algebra{A})$ (as any character of $(a)$ can be extended to $\algebra{A}$), so any character in $\Omega((a))$ is also symmetric. As $a$ is self-adjoint, we have $\chi(a) = \overline{\chi(a^*)} = \overline{\chi(a)}$ and therefore $\chi(a) \in \mathds{R}$ for any $\chi \in \Omega((a))$.
    As $(a)$ is a commutative $^*$-Banach-algebra, we have
    \begin{equation*}
        \sigma_{(a)}(a) \subseteq \{\chi(a) \mid \chi \in \Omega((a)) \} \cup \{0\} \subseteq \mathds{R}\text{.}
    \end{equation*}
    Furthermore, if $a - \lambda \in (a)$ is invertible, it must also be invertible in $\algebra{A} \supseteq (a)$, so $\rho(a)_{(a)} \subseteq \rho_{\algebra{A}}(a)$ and therefore $\sigma_\algebra{A}(a) \subseteq \sigma_{(a)}(a) \subseteq \mathds{R}$.
    \item $\then$ (iii): Let $\Gamma: \algebra{A} \to C(\Omega(\algebra{A})), a \mapsto (\chi \mapsto \chi(a))$ be the Gelfand-transform of $\algebra{A}$.
    We want to prove $\Gamma(a) = \Gamma(a^*)^*$.
    By the Definition of the involution on $C(\Omega(\algebra{A}))$, this is equivalent to $\chi(a) = \overline{\chi(a^*)}$ for any $\chi$ the spectrum and $a \in \algebra{A}$.

    First, let $a \in \algebra{A}$ self-adjoint.
    Then $\overline{\chi(a^*)} = \overline{\chi(a)} = \chi(a)$ as $\chi(a) \in \sigma(a) \subseteq \mathds{R}$.

    If $a \in \algebra{A}$ is not self-adjoint, we can write $a = b + ic$ for self-adjoint elements $b = \frac{a + a^*}{2}$ and $c = \frac{a - a^*}{2i}$ and it follows that
    \begin{equation*}
        \chi(a) = \chi(b + ic) = \chi(b) + i \chi(c) = \overline{\chi(b^*)} + i \overline{\chi(c^*)} = \overline{\chi(b^*) - i \chi(c^*)} = \overline{b^* - i c^*} = \overline{\chi(a^*)}
    \end{equation*}
    and this shows (iii).
    \item $\then$ (i): If $\Gamma$ is a $^*$-homomorphism, then $\Gamma(a^*) = \Gamma(a)^*$ and by the definition of the involution as discussed above this already shows $\chi(a^*) = \overline{\chi(a)}$ for every character $\chi$.
\end{enumerate}



\end{document}